DynamoDbItemEncryptor/src/Index.dfy
@@ -2,14 +2,13 @@
 // SPDX-License-Identifier: Apache-2.0
 
 include "AwsCryptographyDynamoDbItemEncryptorOperations.dfy"
-include "../../StructuredEncryption/src/Index.dfy"
-include "../../private-aws-encryption-sdk-dafny-staging/AwsCryptographicMaterialProviders/src/Index.dfy"
 
 module
   {:extern "Dafny.Aws.Cryptography.DynamoDbItemEncryptor" }
   DynamoDbItemEncryptor refines AbstractAwsCryptographyDynamoDbItemEncryptorService
 {
   import StructuredEncryption
+  import CSE = AwsCryptographyStructuredEncryptionTypes
   import MaterialProviders
   import Operations = AwsCryptographyDynamoDbItemEncryptorOperations
 
@@ -43,26 +42,106 @@ module
   {
     // TODO validation of config input
 
+    // TODO Fix this when the compile bug is fixed (https://t.corp.amazon.com/P78273149)
+    // :- Need(config.keyring.None? || config.cmm.None?, DynamoDbItemEncryptorException(
+    //   message := "Cannot provide both a keyring and a CMM"
+    // ));
+    if !(config.keyring.None? || config.cmm.None?) {
+      return Failure(DynamoDbItemEncryptorException(
+        message := "Cannot provide both a keyring and a CMM"
+      ));
+    }
+    // :- Need(config.keyring.Some? || config.cmm.Some?, DynamoDbItemEncryptorException(
+    //   message := "Must provide eiterh a keyring or a CMM"
+    // ));
+    if !(config.keyring.Some? || config.cmm.Some?) {
+      return Failure(DynamoDbItemEncryptorException(
+        message := "Must provide eiterh a keyring or a CMM"
+      ));
+    }
+    // :- Need(
+    //     && config.partitionKeyName in config.attributeActions
+    //     && config.attributeActions[config.partitionKeyName] == CSE.SIGN_ONLY,
+    //   DynamoDbItemEncryptorException(
+    //     message := "Partition key attribute action MUST be SIGN_ONLY"
+    //   ));
+    if 
+        !(&& config.partitionKeyName in config.attributeActions
+        && config.attributeActions[config.partitionKeyName] == CSE.SIGN_ONLY)
+    {
+      return Failure(DynamoDbItemEncryptorException(
+        message := "Partition key attribute action MUST be SIGN_ONLY"
+      ));
+    }
+    // :- Need(
+    //   (config.sortKeyName.Some? ==>
+    //     && config.sortKeyName.value in config.attributeActions
+    //     && config.attributeActions[config.sortKeyName.value] == CSE.SIGN_ONLY),
+    //   DynamoDbItemEncryptorException(
+    //     message := "Sort key attribute action MUST be SIGN_ONLY"
+    //   ));
+    if !(
+      (config.sortKeyName.Some? ==>
+        && config.sortKeyName.value in config.attributeActions
+        && config.attributeActions[config.sortKeyName.value] == CSE.SIGN_ONLY))
+    {
+      return Failure(DynamoDbItemEncryptorException(
+        message := "Sort key attribute action MUST be SIGN_ONLY"
+      ));
+    }
+
+    var attributeActions' := config.attributeActions;
+    while attributeActions'.Keys != {}
+      invariant forall attribute <- (config.attributeActions - attributeActions'.Keys)
+      :: Operations.ForwardCompatibleAttributeAction(
+          attribute,
+          config.attributeActions[attribute],
+          config.allowedUnauthenticatedAttributes,
+          config.allowedUnauthenticatedAttributePrefix)
+    {
+      var attribute :| attribute in attributeActions';
+      var action := config.attributeActions[attribute];
+      // :- Need(Operations.ForwardCompatibleAttributeAction(
+      //       attribute,
+      //       action,
+      //       config.allowedUnauthenticatedAttributes,
+      //       config.allowedUnauthenticatedAttributePrefix
+      //     ),
+      //     DynamoDbItemEncryptorException(
+      //       message := "Attribute: " + attribute + " configuration not compatible with unauthenticated configuration."
+      //     ));
+      if !(Operations.ForwardCompatibleAttributeAction(
+          attribute,
+          action,
+          config.allowedUnauthenticatedAttributes,
+          config.allowedUnauthenticatedAttributePrefix
+        ))
+      {
+        return Failure(DynamoDbItemEncryptorException(
+          message := "Attribute: " + attribute + " configuration not compatible with unauthenticated configuration."
+        ));
+      }
+      attributeActions' := attributeActions' - {attribute};
+    }
+
     // Create the structured encryption client
     var structuredEncryptionRes := StructuredEncryption.StructuredEncryption();
     var structuredEncryption :- structuredEncryptionRes
       .MapFailure(e => AwsCryptographyStructuredEncryption(e));
 
     // TODO For now just passthrough cmm or wrap keyring with DefaultCMM
-    var maybeCmm := config.cmm;
     var cmm;
-    if (maybeCmm.Some?) {
-      cmm := maybeCmm.value;
+    if (config.cmm.Some?) {
+      cmm := config.cmm.value;
     } else {
-      // TODO for now assume valid input
-      expect config.keyring.Some?;
       var keyring := config.keyring.value;
       var matProv :- expect MaterialProviders.MaterialProviders();
-      cmm :- expect matProv.CreateDefaultCryptographicMaterialsManager(
+      var maybeCmm := matProv.CreateDefaultCryptographicMaterialsManager(
         AwsCryptographyMaterialProvidersTypes.CreateDefaultCryptographicMaterialsManagerInput(
           keyring := keyring
         )
       );
+      cmm :- maybeCmm.MapFailure(e => AwsCryptographyMaterialProviders(e));
     }
 
     var internalConfig := Operations.Config(
